\documentclass[12pt]{article}
 
\usepackage[margin=1in]{geometry} 
\usepackage{amsmath,amsthm,amssymb}
\usepackage{graphicx}
\usepackage{enumerate}
\usepackage{xcolor}
\usepackage{lastpage}
\usepackage[parfill]{parskip}
\usepackage{fancyhdr}

\begin{document}
 
\begin{align*}
\text{Statement to check}&:\\
\sum_{1}^{n}i^3&=\frac{n^2(n+1)^2}{4}\\
\text{Base Case}&: n=1\\
\sum_{1}^{1}i^3&=\frac{1^2(1+1)^2}{4}\\
1^3&= 1 = \frac{1^2(1+1)^2}{4} = 1 \qquad \checkmark\\
\text{Induction Hypothesis}&: n=k\\
\sum_{1}^{k}i^3&=\frac{k^2(k+1)^2}{4}\qquad \checkmark\\
\text{Induction Step}&: n=k+1\\
\sum_{1}^{k+1}i^3&=\frac{(k+1)^2((k+1)+1)^2}{4}\\
\sum_{1}^{k+1}i^3&=\sum_{1}^{k}i^3 + (k+1)^3\\
&=\frac{k^2(k+1)^2}{4} + (k+1)^3\\
&=\frac{k^2(k+1)^2}{4} + \frac{4(k+1)^3}{4}\\
&=\frac{k^2(k+1)^2}{4} + \frac{4(k+1)(k+1)^2}{4}\\
&=\frac{k^2(k+1)^2 + 4(k+1)(k+1)^2}{4}\\
&=\frac{(k+1)^2( k^2 + 4(k+1) )}{4}\\
&=\frac{(k+1)^2( k^2 + 4k + 4) )}{4}\\
&=\frac{(k+1)^2(k + 2)^2}{4}\\
&=\frac{(k+1)^2((k + 1) + 1)^2}{4} \qquad \square
\end{align*} 
\end{document}